Working example with Denvy's reify/reflect + PHOAS

Normalize.v
@@ -6,7 +6,7 @@ From STLCZK Require Import GaloisField.
 From STLCZK Require Import Stlc.
 From STLCZK Require Import R1cs.
 From STLCZK Require Import Ltac.
-
+Require Import Coqprime.elliptic.ZEll.
 From Coq Require Import Vectors.VectorDef.
 From Coq Require Import Init.Nat.
 From Coq Require Import Lists.List.
@@ -19,25 +19,25 @@ Module Normalize(PF: GaloisField).
   Import ListNotations.
   Local Open Scope nat_scope.
 
-  Fixpoint normalize' (e: exp): exp :=
+  Fixpoint normalize' (k: nat)(e: exp): exp :=
     match e with
     | <{ if true then e else _ }> => e
     | <{ if false then _ else e }> => e
     | <{ (\_: t, e1) e2 }> => 
-      open_exp_wrt_exp (normalize' e1) (normalize' e2)
+      open_exp_wrt_exp_rec k (normalize' (S k) e1) (normalize' k e2)
     | <{ \_: _, _ }> => e (** Don't go under binders for HNF, skip heads in normalize'' *)
     | <{ (if c then \_:_, b1 else \_:_, b2) e }> =>
-      let e' := normalize' e in
-      <{ if {normalize' c}
-         then {open_exp_wrt_exp (normalize' b1) e'}
-         else {open_exp_wrt_exp (normalize' b2) e'} }>
+      let e' := normalize' k e in
+      <{ if {normalize' k c}
+         then {open_exp_wrt_exp_rec k (normalize' (S k) b1) e'}
+         else {open_exp_wrt_exp_rec k (normalize' (S k) b2) e'} }>
     | <{ let e1 in e2 }> =>
-      open_exp_wrt_exp (normalize' e2) (normalize' e1)
-    | <{ e1 e2 }> => tm_app (normalize' e1) (normalize' e2)
-    | <{ e1 == e2 }> => <{ {normalize' e1} == {normalize' e2} }>
-    | <{ ! e }> => <{ ! {normalize' e} }>
+      open_exp_wrt_exp_rec k (normalize' (S k) e2) (normalize' k e1)
+    | <{ e1 e2 }> => tm_app (normalize' k e1) (normalize' k e2)
+    | <{ e1 == e2 }> => <{ {normalize' k e1} == {normalize' k e2} }>
+    | <{ ! e }> => <{ ! {normalize' k e} }>
     | <{ if c then e1 else e2 }> =>
-      <{ if {normalize' c} then {normalize' e1} else {normalize' e2} }>
+      <{ if {normalize' k c} then {normalize' k e1} else {normalize' k e2} }>
     | <{ fp f1 + fp f2 }> =>
       let s := pkplus f1 f2 in
       <{ fp s }>
@@ -53,20 +53,27 @@ Module Normalize(PF: GaloisField).
     | <{ _ || true }> => <{ true }>
     | <{ true || _ }> => <{ true }>
     | <{ false || false }> => <{ false }>
-    | tm_binop e1 op e2 => tm_binop (normalize' e1) op (normalize' e2)
+    | tm_binop e1 op e2 => tm_binop (normalize' k e1) op (normalize' k e2)
     | o => o
     end.
 
-  Fixpoint normalize''(e: exp)(gas: nat): exp :=
+  Fixpoint normalize''(e: exp)(k: nat)(gas: nat): option exp :=
     match gas with
-    | 0%nat => e
-    | S g' => normalize'' (normalize' e) g'
+    | 0%nat => None
+    | S g' => let e' := normalize' k e in
+             if eq_exp e' e then
+               Some e'
+             else
+               normalize'' e' k  g'
     end.
 
-  Fixpoint normalize(e: exp)(gas: nat): exp :=
+  Fixpoint normalize(e: exp)(k: nat)(gas: nat): option exp :=
     match e with
-    | <{ \_: t, e }> => <{ \_: t, {normalize e gas} }>
-    | e => normalize'' e gas
+    | <{ \_: t, e }> => match normalize e (S k) gas with
+                       | Some e' => Some <{ \_: t, e' }>
+                       | None => None
+                       end
+    | e => normalize'' e k gas
     end.
   
   Definition foo :=
@@ -79,18 +86,23 @@ Module Normalize(PF: GaloisField).
                ) #1
      }>.
 
+  Definition bar' :=
+    <{ \_: Field,
+           (\_: Field, #0 - #0) #0
+     }>.
+  
   Definition bar :=
     <{ \_: Field,
            let (\_: Field, #0 - #0) in
            #0 #1
      }>.
-  Compute normalize foo 10.
-  Compute normalize bar 10.
+  Compute normalize foo 0 10.
+  Compute normalize bar 0 10.
 
   Lemma normalize_fixpoint: forall e,
-      exists g, normalize e g = e.
+      exists g, g > 0 -> normalize e g = e.
   Proof.
-    induction e; cbn; try (exists 0; reflexivity).
+    induction e; cbn; try (exists 1; reflexivity).
     - destruct IHe.
       exists x.
       rewrite H.
