Phoas.v
@@ -1,0 +1,769 @@
+Require Import Bool.
+Require Import Coqprime.elliptic.ZEll.
+
+(** For F_p *)
+Require Import Coqprime.elliptic.ZEll.
+Require Import Coq.ZArith.Znumtheory.
+Require Import Coq.ZArith.BinInt.
+
+From STLCZK Require Import GaloisField.
+From Coq Require Import Vectors.VectorDef.
+From Coq Require Import Init.Nat.
+
+Set Implicit Arguments.
+
+(** Use the same reified type for the whole development *)
+Inductive type : Type :=
+| TBool: type
+| TInt: type
+| TArrow : type -> type -> type.
+
+Module Stlc_Phoas(Import PF: GaloisField.GaloisField).
+  Import PF.
+
+  Section vars.
+  Variable var : type -> Type.
+
+  Inductive fop : Set := 
+  | op_add : fop
+  | op_sub : fop
+  | op_mul : fop.
+
+  Inductive bop: Set :=
+  | op_and : bop
+  | op_or : bop.
+  
+  Inductive term : type -> Type :=
+  | ECField : Fp -> term TInt
+  | ECBool: bool -> term TBool
+         
+  | EVar : forall t,
+      var t
+      -> term t
+             
+  | EApp : forall t1 t2,
+      term (TArrow t1 t2)
+      -> term t1
+      -> term t2
+  | EAbs : forall t1 t2,
+      (var t1 -> term t2)
+      -> term (TArrow t1 t2)
+
+  (** Control flow *)
+  | EIf: forall t, term TBool ->
+         term t ->
+         term t ->
+         term t
+
+  (** Prim ops *)
+  | EFop: fop ->
+          term TInt ->
+          term TInt ->
+          term TInt
+  | EBop: bop ->
+          term TBool ->
+          term TBool ->
+          term TBool
+  | EFeq: term TInt ->
+          term TInt ->
+          term TBool
+  | ENot: term TBool ->
+          term TBool.
+End vars.
+  
+Arguments EVar [var t].
+Arguments ECField {var}.
+Arguments ECBool {var}.
+Arguments EApp [var t1 t2].
+Arguments EAbs [var t1 t2].
+Arguments EIf [var t].
+Arguments EFop {var}.
+Arguments EBop {var}.
+Arguments EFeq {var}.
+Arguments ENot {var}.
+
+Fixpoint typeDenote (t : type) : Set :=
+  match t with
+  | TBool => bool
+  | TInt => Fp
+  | TArrow t1 t2 => typeDenote t1 -> typeDenote t2
+  end.
+
+Fixpoint termDenote t (e : term typeDenote t) {struct e} : typeDenote t :=
+  match e in (term _ t) return (typeDenote t) with
+    | EVar v => v
+
+    | ECBool t => t
+    | ECField f => f
+
+    | EApp e1 e2 => (termDenote e1) (termDenote e2)
+    | EAbs e' => fun x => termDenote (e' x)
+
+    | EIf c e1 e2 => if (termDenote c) then (termDenote e1) else (termDenote e2)
+
+    | EFop op_add e1 e2 => pkplus (termDenote e1) (termDenote e2)
+    | EFop op_sub e1 e2 => pksub (termDenote e1) (termDenote e2)
+    | EFop op_mul e1 e2 => pkmul (termDenote e1) (termDenote e2)
+    | EBop op_and e1 e2 => andb (termDenote e1) (termDenote e2)
+    | EBop op_or e1 e2 => orb (termDenote e1) (termDenote e2)
+    | EFeq e1 e2 => if eq_field (termDenote e1) (termDenote e2) then true else false
+    | ENot e1 => negb (termDenote e1)
+  end.
+End Stlc_Phoas.
+
+Module DanvyOriginal.
+
+  Definition Int := nat.
+
+  (** The forbidden flag *)
+  Unset Positivity Checking.
+
+  Inductive Term: Type :=
+  | INT: Int -> Term 
+  | ADD: Term -> Term -> Term
+  | APP: Term -> Term -> Term
+  | LAM: (Term -> Term) -> Term.
+
+   Inductive Exp (t: Type) :=
+  | EXP: Term -> Exp t.
+
+  Arguments EXP {t}.
+  Definition int(i: Int): Exp Int :=
+    EXP (INT i).
+  
+  Definition add(a b: Exp Int): Exp Int :=
+    match a, b with
+    | EXP e1, EXP e2 => EXP (ADD e1 e2)
+    end.
+  
+  Definition app a b (f: Exp (a -> b))(o: Exp a) : Exp b :=
+    match f, o with
+    | EXP e1, EXP e2 => EXP (APP e1 e2)
+    end.
+
+  Definition lam a b (f: Exp a -> Exp b): Exp (a -> b) :=
+    EXP (LAM (fun (x: Term) => match f (EXP x) with
+                  | EXP b => b
+                            end)).
+   Definition coerce a (e: Exp (Exp a)): Exp a :=
+    match e with
+    | EXP b => EXP b
+    end.
+
+  Definition uncoerce a (e: Exp a): Exp (Exp a) :=
+    match e with
+    | EXP b => EXP b
+    end.
+      
+  Class Nbe a := {
+    reify: a -> Term;
+    reflect: Term-> a
+                }.
+
+  Instance Nbe_lam a b {na: Nbe a} {nb: Nbe b}: Nbe (a -> b) := {
+    reify v := 
+      LAM (fun x => reify (v (reflect x)));
+    reflect e :=
+      fun x => reflect (APP e (reify x))
+                                                              }.
+
+  Unset Positivity Checking.
+End DanvyOriginal.
+
+Module DanvyPhoas(Import PF: GaloisField.GaloisField).
+  Import PF.
+  
+  Section vars.
+    Variable var : type -> Type.
+
+    Inductive Term: type -> Type :=
+    | INT: Fp -> Term TInt
+    | BOOL: bool -> Term TBool
+    | ADD: Term TInt -> Term TInt -> Term TInt
+    | APP: forall a b, Term (TArrow a b) -> Term a -> Term b
+    | VAR: forall a, var a -> Term a
+    | LAM: forall a b, (var a -> Term b) -> Term (TArrow a b).
+  
+  Fixpoint typeDenote (t : type) : Set :=
+    match t with
+    | TBool => bool
+    | TInt => Fp
+    | TArrow t1 t2 => typeDenote t1 -> typeDenote t2
+    end.
+
+  Class Nbe (t: type) := {
+    reify: typeDenote t -> Term t;
+    reflect: Term t -> typeDenote t
+                }.
+
+  Instance Nbe_lam {a b: type} {na: Nbe a} {nb: Nbe b}: Nbe (TArrow a b) := {
+    reify v := 
+      LAM (fun x => reify (v (reflect (VAR x))));
+    reflect e :=
+      fun x => reflect (APP e (reify x))
+                                                                   }.
+  End vars.
+
+  Arguments VAR [var a].
+  Arguments INT {var}.
+  Arguments BOOL {var}.
+  Arguments ADD {var}.
+  Arguments APP [var a b].
+  Arguments LAM [var a b].
+  (** Maximally insert types in class as well *)
+  Arguments Nbe [var].
+  Arguments Nbe_lam [var a b].
+  
+  Fixpoint termDenote t (e : Term typeDenote t) {struct e} : typeDenote t :=
+    match e in (Term _ t) return (typeDenote t) with
+    | VAR v => v
+    | INT f => f
+    | BOOL v => v
+    | ADD f1 f2 => pkplus (termDenote f1) (termDenote f2)
+    | APP e1 e2 => (termDenote e1) (termDenote e2)
+    | LAM e' => fun x => termDenote (e' x)
+    end.
+
+  Instance Nbe_int : Nbe TInt := {
+    reify v := INT v;
+
+    reflect v := termDenote v;
+                                }.
+  Instance Nbe_bool : Nbe TBool := {
+    reify v := BOOL v;
+    
+    reflect v := termDenote v;
+                                }.
+End DanvyPhoas.
+
+Module DanvyPhoasNf(Import PF: GaloisField.GaloisField).
+  Import PF.
+
+  Section vars.
+    Variable var : type -> Type.
+
+    Fixpoint typeDenote (t : type) : Set :=
+      match t with
+      | TBool => bool
+      | TInt => Fp
+      | TArrow t1 t2 => typeDenote t1 -> typeDenote t2
+      end.
+
+    (** Danvy paper:
+        data NfTerm = COERCE AtTerm | LAM (AtTerm → NfTerm)
+        data AtTerm = APP AtTerm NfTerm
+      + PHOAS
+     *)
+    Inductive NfTerm: type -> Type :=
+    | NCOERCE: forall t, AtTerm t -> NfTerm t
+    | LAM: forall a b, (var a -> NfTerm b) -> NfTerm (TArrow a b)
+    with AtTerm: type -> Type :=
+    | VAR: forall a, var a -> AtTerm a (** Is var correctly an AtTerm ? *)
+    | APP: forall a b, AtTerm (TArrow a b) -> NfTerm a -> AtTerm b
+    | PCOERCE: forall t, PrTerm t -> AtTerm t
+    | ADD: AtTerm TInt -> AtTerm TInt -> AtTerm TInt
+    with PrTerm: type -> Type :=
+    | INT: Fp -> PrTerm TInt
+    | BOOL: bool -> PrTerm TBool.
+
+    Class Nbe (t: type) := {
+      reify: typeDenote t -> NfTerm t;
+      reflect: AtTerm t -> typeDenote t
+                          }.
+
+    Instance Nbe_lam {a b: type} {na: Nbe a} {nb: Nbe b}: Nbe (TArrow a b) := {
+      reify v := 
+        LAM (fun x => reify (v (reflect (VAR x))));
+      reflect e :=
+        fun x => reflect (APP e (reify x))
+                                                                   }.
+  End vars.
+
+  Arguments VAR [var a].
+  Arguments INT {var}.
+  Arguments BOOL {var}.
+  Arguments ADD {var}.
+  Arguments NCOERCE [var t].
+  Arguments APP [var a b].
+  Arguments PCOERCE [var t].
+  Arguments LAM [var a b].
+  (** Maximally insert types in class as well *)
+  Arguments Nbe [var].
+  Arguments Nbe_lam [var a b].
+
+  (** Danvy's nf and at + primitive terms Int and Bool *)
+  Fixpoint nfTermDenote t (e : NfTerm typeDenote t) {struct e} : typeDenote t :=
+    match e in (NfTerm _ t) return (typeDenote t) with
+    | NCOERCE a => atTermDenote a
+    | LAM f => fun x => nfTermDenote (f x)
+    end
+  with atTermDenote t (e: AtTerm typeDenote t) {struct e}: typeDenote t :=
+    match e in (AtTerm _ t) return (typeDenote t) with
+    | APP e1 e2 => (atTermDenote e1) (nfTermDenote e2)
+    | VAR v => v
+    | PCOERCE p => prTermDenote p
+    | ADD f1 f2 => pkplus (atTermDenote f1) (atTermDenote f2)
+    end
+  with prTermDenote t (e: PrTerm typeDenote t) {struct e}: typeDenote t :=
+    match e in (PrTerm _ t) return (typeDenote t) with
+    | INT v => v
+    | BOOL v => v
+    end.
+
+  Instance Nbe_int : Nbe TInt := {
+    reify v := NCOERCE (PCOERCE (INT v));
+
+    reflect v := atTermDenote v;
+                                }.
+
+  Instance Nbe_bool : Nbe TBool := {
+    reify v := NCOERCE (PCOERCE (BOOL v));
+    
+    reflect v := atTermDenote v;
+                                }.
+End DanvyPhoasNf.
+
+(** ScratchPAD *)         
+Fixpoint termDenoteReify t (x : typeDenote t) : term typeDenote t :=
+  match t return (_ = _ -> term typeDenote t) with
+  | TBool => (fun _: t = x => ECBool x)
+  | TField => ECField x
+  | TArrow t1 t2 => EAbs (fun v => x (termDenote t1 (EVar v)))
+  end.
+
+Definition Term t := forall var, term var t.
+Definition TermDenote t (e : Term t) := termDenote (e _).
+
+Fixpoint closed_value(t: type): Term t :=
+  match t with
+  | TField => fun _ => ECField (0:%p)
+  | TBool => fun _ => ECBool true
+  | TArrow _ t2 => fun _ => EAbs (fun _ => @closed_value t2 _)
+  end.
+
+Definition input_type(t: type): type :=
+  match t with
+  | TArrow t1 t2 => t1
+  | _ => t
+  end.
+
+Fixpoint closed t (e: term _ t): bool :=
+  match e with
+  | EVar v => true
+  | ECBool _ => false
+  | ECField _ => false
+  | EApp e1 e2 => andb (closed e1) (closed e2)
+  | EIf c e1 e2 => andb (closed c) (andb (closed e1) (closed e2))
+  | EFop _ e1 e2 => andb (closed e1) (closed e2)
+  | EBop _ e1 e2 => andb (closed e1) (closed e2)
+  | EFeq e1 e2 => andb (closed e1) (closed e2)
+  | ENot e => closed e
+  | EAbs e' => closed (e' (closed_value ))
+  end.
+
+Definition value(t: type): Term t -> Prop :=
+  match t with
+  | TField => fun u => exists f: Fp, forall v, u v = ECField f
+  | TBool => fun u => exists b: bool, forall v, u v = ECBool b
+  | TArrow t1 t2 => fun u => forall v, exists f: v t1 -> term v t2, u v = EAbs f
+  end.
+
+Fixpoint computation(t: type): Term t -> Prop :=
+  fun m => exists v, termDenote m = v
+
+                    
+
+Inductive fot: type -> Prop :=
+| FotB: fot TBool
+| FotF: fot TField.
+
+Definition fo_term(t: type) := { e: Term t | fot t }.
+
+End Stlc_Phoas.
+
+Module Stlc(Import PF: GaloisField.GaloisField).
+  Import PF.
+  Include Stlc_Phoas PF.
+  
+  Declare Custom Entry stlc_ty.
+  Declare Custom Entry stlc.
+  
+  Notation "'fp' n" := (ECField n) (in custom stlc at level 0).
+  Notation "'true'"  := true (at level 1).
+  Notation "'true'" := (ECBool true) (in custom stlc at level 0).
+  Notation "'false'"  := false (at level 1).
+  Notation "'false'" := (ECBool false) (in custom stlc at level 0).
+  Notation "<{ e }>" := e (e custom stlc at level 99).
+  Notation "<{{ e }}>" := e (e custom stlc_ty at level 99).
+  Notation "( x )" := x (in custom stlc, x at level 99).
+  Notation "( x )" := x (in custom stlc_ty, x at level 99).
+  Notation "x" := x (in custom stlc at level 0, x constr at level 0).
+  Notation "x" := x (in custom stlc_ty at level 0, x constr at level 0).  
+  Notation "x y" := (EApp x y) (in custom stlc at level 1, left associativity).
+  
+  Notation "\ x , y" :=
+    (EAbs (fun x => y)) (in custom stlc at level 90,
+                 y custom stlc at level 80,
+                 left associativity).
+  Notation "\_ , y" :=
+    (EAbs (fun _ => y)) (in custom stlc at level 90,
+                 y custom stlc at level 80,
+                 left associativity).
+  
+  Notation "# n" := (EVar n) (in custom stlc at level 0).
+  Notation "{ x }" := x (in custom stlc at level 1, x constr).
+  Notation "S -> T" := (TArrow S T) (in custom stlc_ty at level 2, right associativity).
+  Notation "'Field'" := TField (in custom stlc_ty at level 0).
+  Notation "'Bool'" := TBool (in custom stlc_ty at level 0).
+  
+  Notation "x + y" := (EFop op_add x y) (in custom stlc at level 2,
+                                            left associativity).
+  Notation "x - y" := (EFop op_sub x y) (in custom stlc at level 2,
+                                            left associativity).
+  Notation "x * y" := (EFop op_mul x y) (in custom stlc at level 1,
+                                            left associativity).
+  Notation "x && y" := (EBop op_and x y) (in custom stlc at level 4,
+                                             left associativity).
+  Notation "x || y" := (EBop op_or x  y) (in custom stlc at level 4,
+                                             left associativity).
+  Notation "x == y" := (EFeq x y) (in custom stlc at level 3,
+                                      left associativity).
+  Notation "! x " := (ENot x) (in custom stlc at level 3).
+
+  Notation "'if' x 'then' y 'else' z" :=
+    (EIf x y z) (in custom stlc at level 89,
+                    x custom stlc at level 99,
+                    y custom stlc at level 99,
+                    z custom stlc at level 99,
+                    left associativity).
+
+Definition fals : Term <{{ Bool }}> := fun _ => <{ false }>.
+Eval compute in TermDenote fals.
+
+Definition tru : Term <{{ Bool }}> := fun _ => <{ true }>.
+Eval compute in TermDenote tru.
+
+Definition ident : Term <{{ Bool -> Bool }}> := fun _ => <{ \x , #x }>.
+Eval compute in (TermDenote ident).
+
+Definition fals_again : Term Bool := fun _ => ident _ @ fals _.
+Eval compute in TermDenote fals_again.
+
+Definition first : Term (Bool --> Bool --> Bool) := fun _ => \x, \y, #x.
+Eval compute in TermDenote first.
+
+Definition second : Term (Bool --> Bool --> Bool) := fun _ => \x, \y, #y.
+Eval compute in TermDenote second.
+
+Definition test_first : Term Bool := fun _ => first _ @ fals _ @ tru _.
+Eval compute in TermDenote test_first.
+
+Definition test_second : Term Bool := fun _ => second _ @ fals _ @ tru _.
+Eval compute in TermDenote test_second.
+
+Definition app : Term ((Bool --> Bool) --> Bool --> Bool) :=
+  fun _ => \f, \x, #f @ #x.
+Eval compute in TermDenote app.
+
+Definition fals_again2 : Term Bool := fun _ => app _ @ ident _ @ fals _.
+Eval compute in TermDenote fals_again2.        
+
+Section normalize.
+  Definition fo: Type -> Prop :=
+    | FoBool bool_scope
+  Fixpoint normalize a Term a -> 
+
+(** CPS *)
+Inductive ptype : Type :=
+| PBool : ptype
+| PCont : ptype -> ptype
+| PUnit : ptype
+| PProd : ptype -> ptype -> ptype.
+
+Notation "'Bool'" := PBool : cps_scope.
+Notation "t --->" := (PCont t) (at level 61) : cps_scope.
+Notation "'Unit'" := PUnit : cps_scope.
+Infix "**" := PProd (right associativity, at level 60) : cps_scope.
+
+Bind Scope cps_scope with ptype.
+Delimit Scope cps_scope with cps.
+
+Section vars.
+  Variable var : ptype -> Type.
+
+  Variable result : ptype.
+
+  Inductive pterm : Type :=
+  | PHalt :
+    var result
+    -> pterm
+  | PApp : forall t,
+    var (t --->)
+    -> var t
+    -> pterm
+  | PBind : forall t,
+    pprimop t
+    -> (var t -> pterm)
+    -> pterm
+
+  with pprimop : ptype -> Type :=
+  | PVar : forall t,
+    var t
+    -> pprimop t
+    
+  | PTrue : pprimop Bool
+  | PFalse : pprimop Bool
+    
+  | PAbs : forall t,
+    (var t -> pterm)
+    -> pprimop (t --->)
+
+  | PPair : forall t1 t2,
+    var t1
+    -> var t2
+    -> pprimop (t1 ** t2)
+  | PFst : forall t1 t2,
+    var (t1 ** t2)
+    -> pprimop t1
+  | PSnd : forall t1 t2,
+    var (t1 ** t2)
+    -> pprimop t2.
+  Check pterm_ind.
+End vars.
+
+Arguments PHalt [var result].
+Arguments PApp [var result t].
+Arguments PBind [var result t].
+
+Arguments PVar [var result t].
+Arguments PTrue {var result}.
+Arguments PFalse {var result}.
+Arguments PAbs [var result t].
+Arguments PPair [var result t1 t2].
+Arguments PFst [var result t1 t2].
+Arguments PSnd [var result t1 t2].
+
+Notation "'Halt' x" := (PHalt x) (no associativity, at level 75) : cps_scope.
+Infix "@@" := PApp (no associativity, at level 75) : cps_scope.
+Notation "x <- p ; e" := (PBind p (fun x => e))
+  (right associativity, at level 76, p at next level) : cps_scope.
+Notation "! <- p ; e" := (PBind p (fun _ => e))
+  (right associativity, at level 76, p at next level) : cps_scope.
+
+Notation "# v" := (PVar v) (at level 70) : cps_scope.
+
+Notation "'Tru'" := PTrue : cps_scope.
+Notation "'Fals'" := PFalse : cps_scope.
+
+Notation "\ x , e" := (PAbs (fun x => e)) (at level 78) : cps_scope.
+Notation "\ ! , e" := (PAbs (fun _ => e)) (at level 78) : cps_scope.
+
+Notation "[ x1 , x2 ]" := (PPair x1 x2) (at level 73) : cps_scope.
+Notation "#1 x" := (PFst x) (at level 72) : cps_scope.
+Notation "#2 x" := (PSnd x) (at level 72) : cps_scope.
+
+Bind Scope cps_scope with pterm pprimop.
+
+Local Open Scope cps_scope.
+
+Fixpoint ptypeDenote (t : ptype) : Set :=
+  match t with
+    | Bool => bool
+    | t' ---> => ptypeDenote t' -> bool
+    | Unit => unit
+    | t1 ** t2 => (ptypeDenote t1 * ptypeDenote t2)%type
+  end.
+
+Fixpoint ptermDenote result (e : pterm ptypeDenote result) (k : ptypeDenote result -> bool)
+  {struct e} : bool :=
+  match e with
+    | PHalt v => k v
+    | PApp f x => f x
+    | PBind p x => ptermDenote (x (pprimopDenote p k)) k
+  end
+
+with pprimopDenote result t (p : pprimop ptypeDenote result t) (k : ptypeDenote result -> bool)
+  {struct p} : ptypeDenote t :=
+  match p in (pprimop _ _ t) return (ptypeDenote t) with
+    | PVar v => v
+
+    | PTrue => true
+    | PFalse => false
+
+    | PAbs e => fun x => ptermDenote (e x) k
+
+    | PPair v1 v2 => (v1, v2)
+    | PFst v => fst v
+    | PSnd v => snd v
+  end.
+
+Definition Pterm result := forall var, pterm var result.
+Definition Pprimop result t := forall var, pprimop var result t.
+Definition PtermDenote result (e : Pterm result) := ptermDenote (e _).
+Definition PprimopDenote result t (p : Pprimop result t) := pprimopDenote (p _).
+                                                               
+(** * CPS translation *)
+
+(** ** Translating types *)
+
+Fixpoint cpsType (t : type) : ptype :=
+  match t with
+    | Bool => Bool%cps
+    | t1 --> t2 => (cpsType t1 ** (cpsType t2 --->) --->)%cps
+  end%source.
+
+(** ** Translating terms *)
+
+Section splice.
+  Local Open Scope cps_scope.
+
+  Fixpoint splice (var : ptype -> Type) (result1 result2 : ptype) (e1 : pterm var result1) (e2 : var result1 -> pterm var result2) {struct e1} : pterm var result2 :=
+    match e1 with
+      | PHalt v => e2 v
+      | PApp f x => f @@ x
+      | PBind p e' => x <- splicePrim p e2; splice (e' x) e2
+    end
+
+  with splicePrim (var : ptype -> Type) (result1 result2 : ptype) t (p : pprimop var result1 t) (e2 : var result1 -> pterm var result2) {struct p} : pprimop var result2 t :=
+    match p in (pprimop _ _ t) return (pprimop var result2 t) with
+      | PVar v => #v
+
+      | PTrue => Tru
+      | PFalse => Fals
+
+      | PAbs e => \x, splice (e x) e2
+
+      | PPair v1 v2 => [v1, v2]
+
+      | PFst v => #1 v
+      | PSnd v => #2 v
+    end.
+End splice.
+
+Notation "x <-- e1 ; e2" := (splice e1 (fun x => e2))
+  (right associativity, at level 76, e1 at next level) : cps_scope.
+Notation "! <-- e1 ; e2" := (splice e1 (fun _ => e2))
+  (right associativity, at level 76, e1 at next level) : cps_scope.
+
+Section cpsTerm.
+  Variable var : ptype -> Type.
+
+  Notation var' := (fun t => var (cpsType t)).
+
+  Local Open Scope cps_scope.
+
+  Fixpoint cpsTerm t (e : term var' t) {struct e} : pterm var (cpsType t) :=
+    match e in (term _ t) return (pterm var (cpsType t)) with
+      | EVar v => PHalt (var := var) v
+
+      | ETrue => x <- Tru; Halt x
+      | EFalse => x <- Fals; Halt x
+
+      | EApp e1 e2 =>
+        f <-- cpsTerm e1;
+        x <-- cpsTerm e2;
+        k <- \r, PHalt (var := var) r;
+        p <- [x, k];
+        f @@ p
+      | EAbs e' =>
+        f <- PAbs (var := var) (fun p =>
+          x <- #1 p;
+          k <- #2 p;
+          r <-- cpsTerm (e' x);
+          k @@ r);
+        Halt f
+    end.
+End cpsTerm.
+
+Arguments cpsTerm [var t].
+Definition CpsTerm t (E : Term t) : Pterm (cpsType t) := fun _ => cpsTerm (E _).
+
+(** * Correctness *)
+
+(**
+pterm_ind
+     : forall P : pterm -> Prop,
+       (forall v : var result, P (PHalt v)) ->
+       (forall (t : ptype) (v : var (t --->)) (v0 : var t), P (PApp v v0)) ->
+       (forall (t : ptype) (p : pprimop t) (p0 : var t -> pterm),
+        (forall v : var t, P (p0 v)) -> P (PBind p p0)) -> forall p : pterm, P p
+*)
+Scheme pterm_mut := Induction for pterm Sort Prop
+with pprimop_mut := Induction for pprimop Sort Prop.
+
+Section splice_correct.
+  Variables result1 result2 : ptype.
+
+  Variable e2 : ptypeDenote result1 -> pterm ptypeDenote result2.  
+
+  Theorem splice_correct : forall e1 k,
+    ptermDenote (splice e1 e2) k
+    = ptermDenote e1 (fun r => ptermDenote (e2 r) k).
+    apply (pterm_mut
+      (fun e1 => forall k,
+        ptermDenote (splice e1 e2) k
+        = ptermDenote e1 (fun r => ptermDenote (e2 r) k))
+      (fun t p => forall k,
+        pprimopDenote (splicePrim p e2) k
+        = pprimopDenote p (fun r => ptermDenote (e2 r) k))); auto.
+    equation.
+  Qed.
+End splice_correct.
+
+Fixpoint lr (t : type) : typeDenote t -> ptypeDenote (cpsType t) -> Prop :=
+  match t return (typeDenote t -> ptypeDenote (cpsType t) -> Prop) with
+    | TBool => fun n1 n2 => n1 = n2
+    | TArrow t1 t2 => fun f1 f2 =>
+      forall x1 x2, lr _ x1 x2
+        -> forall k, exists r,
+          f2 (x2, k) = k r
+          /\ lr _ (f1 x1) r
+  end.
+
+Lemma cpsTerm_correct : forall G t (e1 : term _ t) (e2 : term _ t),
+  term_equiv G e1 e2
+  -> (forall t v1 v2, In (vars (v1, v2)) G -> lr t v1 v2)
+  -> forall k, exists r,
+    ptermDenote (cpsTerm e2) k = k r
+    /\ lr t (termDenote e1) r.
+  Hint Rewrite splice_correct : ltamer.
+
+  Ltac my_changer :=
+    match goal with
+      [ H : (forall (t : _) (v1 : _) (v2 : _), vars _ = vars _ \/ In _ _ -> _) -> _ |- _ ] =>
+      match typeof H with
+        | ?P -> _ =>
+          assert P; [intros; push_vars; intuition; fail 2
+            | idtac]
+      end
+    end.
+
+  Ltac my_simpler := repeat progress (equation; fold ptypeDenote in *;
+    fold cpsType in *; try my_changer).
+
+  Ltac my_chooser T k :=
+    match T with
+      | bool => fail 1
+      | type => fail 1
+      | ctxt _ _ => fail 1
+      | _ => default_chooser T k
+    end.
+
+  induction 1; matching my_simpler my_chooser; eauto.
+Qed.
+
+Theorem CpsTerm_correct : forall t (E : Term t),
+  forall k, exists r,
+    PtermDenote (CpsTerm E) k = k r
+    /\ lr t (TermDenote E) r.
+  unfold PtermDenote, TermDenote, CpsTerm; simpl; intros.
+  eapply (cpsTerm_correct (G := nil)); simpl; intuition.
+  apply Term_equiv.
+Qed.
+
+Theorem CpsTerm_correct_bool : forall (E : Term TBool),
+  forall k, PtermDenote (CpsTerm E) k = k (TermDenote E).
+  intros.
+  generalize (CpsTerm_correct E k); firstorder congruence.
+Qed.
+                                          
